numLib.sml : performance bug fixed in ADD_CONV
prim_recScript : Basic wellfoundedness theorems about numbers added.

numeralScript.sml : minor tweaks to accomodate change to prim_recScript

NonRecSize : this is a structure that installs `size` functions in
             TypeBase.theTypeBase for non-recursive types. This
             structure basically keeps sums, products, and options
             from depending on nums (and vice versa) in the theory
             hierarchy.

src/num/NonRecSize.sml
@@ -1,0 +1,57 @@
+(*---------------------------------------------------------------------------*
+ * Setting information for types.                                            *
+ *                                                                           *
+ * Here we fill in the "size" entries in theTypeBase for some types that     *
+ * are non-recursive and built before numbers.                               *
+ *---------------------------------------------------------------------------*)
+
+structure NonRecSize =
+struct
+
+open HolKernel basicHol90Lib Parse;
+local open pairTheory sumTheory optionTheory in end;
+
+infix THEN THENC THENL |-> ORELSE;
+infixr -->;
+
+
+local
+  val prod_size_info =
+       (Parse.Term`\f g. UNCURRY(\(x:'a) (y:'b). f x + g y)`,
+        pairTheory.UNCURRY_DEF)
+  val prod_info' = TypeBase.put_size prod_size_info 
+                      (Option.valOf(TypeBase.read"prod"))
+
+  val bool_info = Option.valOf(TypeBase.read "bool")
+  val bool_case_rw = prove(Term`!x y. bool_case x x y = (x:'a)`,
+    REPEAT GEN_TAC
+      THEN BOOL_CASES_TAC (Term`y:bool`)
+     THEN Rewrite.ASM_REWRITE_TAC[boolTheory.bool_case_DEF]);
+  val bool_size_info = (Term`bool_case 0 0`, bool_case_rw)
+  val bool_info' = TypeBase.put_size bool_size_info bool_info
+
+  val sum_info = Option.valOf(TypeBase.read "sum")
+  val sum_case = #const(Term.const_decl "sum_case")
+  val num = Type`:num`
+  val sum_case_into_num = inst [alpha |-> num] sum_case
+  val f = mk_var{Name="f",Ty=beta-->num}
+  val g = mk_var{Name="g",Ty=mk_vartype"'c" --> num}
+  val s = mk_var{Name="s",Ty=mk_type{Tyop="sum",Args=[beta, mk_vartype "'c"]}}
+  val tm = list_mk_abs ([f,g,s], list_mk_comb(sum_case_into_num,[f,g,s]))
+  val sum_size_info = (tm,sumTheory.sum_case_def)
+  val sum_info' = TypeBase.put_size sum_size_info sum_info
+
+  val option_info = Option.valOf(TypeBase.read "option")
+  val option_size_info =
+       (Parse.Term`\f. option_case 0 (\x:'a. SUC (f x))`,
+        optionTheory.option_case_def)
+  val option_info' = TypeBase.put_size option_size_info option_info
+
+in
+   val _ = TypeBase.write bool_info'
+   val _ = TypeBase.write prod_info'
+   val _ = TypeBase.write option_info'
+   val _ = TypeBase.write sum_info'
+end
+
+end;
